Aesop/RuleTac/Descr.lean
@@ -1,0 +1,33 @@
+import Aesop.RuleTac.Basic
+import Aesop.Forward.Match.Types
+
+open Lean Lean.Meta
+
+namespace Aesop
+
+inductive RuleTacDescr
+  | apply (term : RuleTerm) (md : TransparencyMode) (pat? : Option RulePattern)
+  | constructors (constructorNames : Array Name) (md : TransparencyMode)
+  | forward (term : RuleTerm) (pat? : Option RulePattern)
+      (immediate : UnorderedArraySet Nat) (isDestruct : Bool)
+      (md : TransparencyMode)
+  | cases (target : CasesTarget) (md : TransparencyMode)
+      (isRecursiveType : Bool) (ctorNames : Array CtorNames)
+  | tacticM (decl : Name)
+  | ruleTac (decl : Name)
+  | tacGen (decl : Name)
+  | singleRuleTac (decl : Name)
+  | tacticStx (stx : Syntax)
+  | preprocess
+  | forwardMatch (m : ForwardRuleMatch)
+  deriving Inhabited
+
+namespace RuleTacDescr
+
+def forwardRuleMatch? : RuleTacDescr → Option ForwardRuleMatch
+  | forwardMatch m => m
+  | _ => none
+
+end RuleTacDescr
+
+end Aesop
